\documentclass{article}

\usepackage{amssymb,amsmath}

\begin{document}

\section{Ex7 : Task2:}
Find a Fourier series for $f (x) = x^2$ and use it to derive another series for $\pi^2$ and a series
for $\pi^4$.

\subsection{Fourier Series for $f(x) = x^2$}

\[
f(-x) = f(x) \Rightarrow \text{even} \Rightarrow b_n=0\forall n
\]

\begin{align}
a_n &= \frac{1}{\pi} \int_{-\pi}^\pi {f(x) \cos{nx} dx} \\
  &= \frac{1}{\pi} \int_{-\pi}^\pi {x^2 \cos{nx} dx} \\
	&= \frac{1}{\pi} \left[ \frac{n^2x^2-2\sin{nx} + 2nx\cos{nx}}{n^3} \right]_{-\pi}^\pi \\
	&= \frac{1}{\pi} \left[ \frac{2n\pi\cos{n\pi}}{n^3} + \frac{2n\pi\cos{n\pi}}{n^3} \right] \\
	&= \frac{1}{\pi n^3}4n\pi\underbrace{\cos{n\pi}}_{+1 \text{for n even}; -1 \text{for n odd}}\\
	&= (-1)^n \frac{4}{n^2}
\end{align}

\begin{align}
a_0 &= \frac{1}{\pi} \int_{-\pi}^\pi {f(x) dx} \\
  &= \frac{1}{\pi} \int_{-\pi}^\pi {x^2 dx} \\
	&= \frac{1}{\pi} \left[ \frac{1}{3}x^3 \right]_{-\pi}^\pi \\
	&= \frac{2\pi^2}{3}
\end{align}

\begin{align}
\Rightarrow f(x) &= \frac{2\pi^2}{3} + 4 \sum_{n\in N}{(-1)}^n \frac{\cos{nx}}{n^2}
\end{align}

\subsection{Series for $\pi^2$:}

\begin{align}
f(0) &= 0 \\
     &= \frac{2\pi^2}{3} + 4 \sum_{n\in N}{\frac{(-1)^n}{n^2}}
\end{align}

\begin{align}
	\Rightarrow \frac{2\pi^2}{3} &=  - 4 \sum_{n\in N}{\frac{(-1)^n}{n^2}}\\
	\Rightarrow \pi^2 &=  6 \sum_{n\in N}{\frac{(-1)^{(n+1)}}{n^2}} \\
	\Rightarrow \pi^2 &=  \frac{6}{1} - \frac{6}{4} + \frac{6}{9} - \frac{6}{16} \pm \ldots
\end{align}

\subsection{Series for $\pi^4$:}
using Parseval relation

\begin{align}
	\frac{1}{\pi} \int_{-\pi}^\pi {f^2(x) dx} = \frac{1}{2} a_0^2 + \sum_{n=1}^\infty (a_n^2 + b_n^2)
	\label{eq:pars}
\end{align}

\begin{align}
	\Rightarrow \frac{1}{\pi} \int_{-\pi}^\pi {f^2(x) dx} &=  \frac{1}{\pi} \int_{-\pi}^\pi {(x^2)^2 dx}\\
		&= \frac{1}{\pi} \left[ \frac{x^5}{5} \right]_{-\pi}^\pi\\
		&= \frac{2\pi^4}{5}\\
		&\overbrace{=}^{\eqref{eq:pars}} \frac{1}{2} a_0^2 + \sum_{n=1}^\infty (a_n^2 + \underbrace{b_n^2}_{=0})\\
		&= \frac{1}{2} \left(\frac{2\pi^2}{3}\right)^2 + \sum_{n=1}^\infty \left( \frac{4(-1)^n}{n^2} \right)^2\\
		&= \frac{2\pi^4}{9} + \sum_{n=1}^\infty \frac{16}{n^4}
\end{align}

\begin{align}
	\Rightarrow \frac{2\pi^4}{5} &= \frac{2\pi^4}{9} + \sum_{n=1}^\infty \frac{16}{n^4} \\
	\Rightarrow \frac{8\pi^4}{45} &= \sum_{n=1}^\infty \frac{16}{n^4} \\
	\Rightarrow \pi^4 &= 90 \sum_{n=1}^\infty \frac{1}{n^4} \\
	\Rightarrow \pi^4 &= 90 \sum_{n=1}^\infty \frac{1}{n^4}
\end{align}



\end{document}